More notes on run-oriented loop rule proof for partial correctness, nicer loop rule proof for total correctness

src/theory/abstract_hoare_logic/abstract_hoare_logicScript.sml
@@ -172,7 +172,8 @@ val abstract_jgmt_def = Define `
     (post ms'))
 `;
 
-
+(* TODO: Can this be rephrased better?
+ * Antecedents guarantee swapping transition system of ANY contract. *)
 val abstract_weak_model_comp_rule_thm = store_thm("abstract_weak_model_comp_rule_thm",
   ``!m n l ls pre post.
     weak_model m ==>
@@ -203,9 +204,9 @@ val abstract_case_rule_thm = prove(``
   abstract_jgmt m l ls pre post
 ``,
 
-REPEAT STRIP_TAC >>
-FULL_SIMP_TAC std_ss [abstract_jgmt_def] >>
-METIS_TAC []
+rpt strip_tac >>
+fs [abstract_jgmt_def] >>
+metis_tac []
 );
 
 val abstract_conseq_rule_thm =
@@ -219,9 +220,9 @@ val abstract_conseq_rule_thm =
     abstract_jgmt m l ls pre2 post2
   ``,
 
-SIMP_TAC std_ss [abstract_jgmt_def] >>
-REPEAT STRIP_TAC >>
-METIS_TAC [weak_pc_in_thm]
+rpt strip_tac >>
+fs [abstract_jgmt_def] >>
+metis_tac [weak_pc_in_thm]
 );
 
 
@@ -246,27 +247,29 @@ val abstract_seq_rule_thm = store_thm("abstract_seq_rule_thm",
   ``!m l ls1 ls2 pre post.
     weak_model m ==>
     abstract_jgmt m l (ls1 UNION ls2) pre post ==>
-    (!l1. (l1 IN ls1) ==>
-    (abstract_jgmt m l1 ls2 post post)) ==>
+    (!l1.
+     l1 IN ls1 ==>
+     abstract_jgmt m l1 ls2 post post
+    ) ==>
     abstract_jgmt m l ls2 pre post``,
 
 REPEAT STRIP_TAC >>
 SIMP_TAC std_ss [abstract_jgmt_def] >>
 REPEAT STRIP_TAC >>
-PAT_X_ASSUM ``(abstract_jgmt m l (ls1 UNION ls2) pre  post)``
+PAT_X_ASSUM ``abstract_jgmt m l (ls1 UNION ls2) pre post``
               (fn thm => ASSUME_TAC (SIMP_RULE std_ss [abstract_jgmt_def] thm)) >>
-QSPECL_X_ASSUM ``!x.P`` [`ms`] >>
+QSPECL_X_ASSUM ``!ms. _`` [`ms`] >>
 REV_FULL_SIMP_TAC std_ss [] >>
-Cases_on `(m.pc ms') IN ls2` >- (
+Cases_on `m.pc ms' IN ls2` >- (
   METIS_TAC [weak_union2_thm]
 ) >>
-Q.SUBGOAL_THEN `(m.pc ms') IN ls1` ASSUME_TAC >- (
+subgoal `m.pc ms' IN ls1` >- (
   METIS_TAC [weak_union_thm, weak_pc_in_thm]
 ) >>
 QSPECL_X_ASSUM  ``!l1. _`` [`m.pc ms'`] >>
 REV_FULL_SIMP_TAC std_ss [abstract_jgmt_def] >>
 QSPECL_X_ASSUM  ``!m. _`` [`ms'`] >>
-REV_FULL_SIMP_TAC std_ss[] >>
+REV_FULL_SIMP_TAC std_ss [] >>
 ASSUME_TAC (Q.SPECL [`m`] weak_comp_thm) >>
 METIS_TAC []
 );
@@ -325,123 +328,105 @@ val (loop_fun_eqns, loop_fun_ind) = Defn.tprove(loop_fun_defn,
 
 val abstract_loop_jgmt_def = Define `
   abstract_loop_jgmt m l le invariant C1 var =
-    ((~(l IN le)) /\
-    (!x. (abstract_jgmt m l ({l} UNION le) (\ms. (invariant ms) /\ (C1 ms) /\ ((var ms) = x:num))
-         (\ms.(((m.pc ms)=l) /\ (invariant ms) /\ ((var ms) < x) /\ ((var ms) >= 0))))))
+    (~(l IN le) /\
+    !x. abstract_jgmt m l ({l} UNION le) (\ms. invariant ms /\ C1 ms /\ var ms = x:num)
+          (\ms. m.pc ms = l /\ invariant ms /\ var ms < x /\ var ms >= 0))
 `;
 
-val inductive_invariant_goal =
-(fst o dest_imp o concl ) (
-  Q.SPEC `(\m ms var l le invariant C1.
+(* TODO: Try removing C1 from the last conjunct, see what happens? *)
+val loop_fun_ind_spec =
+  Q.SPEC `\m ms var l le invariant C1.
 	   weak_model m ==>
 	   abstract_loop_jgmt m l le invariant C1 var ==>
-	   abstract_jgmt m l le (\ms. (invariant ms) /\ (~(C1 ms))) post ==>
-	   ((invariant ms) /\ ((m.pc ms) = l) /\ (C1 ms)) ==>
-	   (?ms'. ((m.weak ms le ms') /\ (post ms'))))`
-  loop_fun_ind
-);
+	   abstract_jgmt m l le (\ms. invariant ms /\ ~C1 ms) post ==>
+	   (invariant ms /\ m.pc ms = l /\ C1 ms) ==>
+	   (?ms'. m.weak ms le ms' /\ post ms')` loop_fun_ind;
+
+
+val inductive_invariant_goal = fst $ dest_imp $ concl loop_fun_ind_spec;
 
 
 val inductive_invariant = prove(``
-^inductive_invariant_goal
+  ^inductive_invariant_goal
 ``,
 
-REPEAT STRIP_TAC >>
-FULL_SIMP_TAC std_ss [] >>
-REPEAT STRIP_TAC >>
-(* We first prove that one iteration works *)
-SUBGOAL_THEN ``(loop_step m ms var l le invariant C1) <> {}`` ASSUME_TAC  >- (
-  SIMP_TAC std_ss [loop_step_def, LET_DEF] >>
-  FULL_SIMP_TAC std_ss [abstract_loop_jgmt_def] >>
-  QSPECL_X_ASSUM ``!x. _`` [`(var (ms)):num`] >>
-  FULL_SIMP_TAC std_ss [abstract_jgmt_def] >>
-  QSPECL_X_ASSUM ``!x. _`` [`ms`] >>
-  REV_FULL_SIMP_TAC std_ss [] >>
-  FULL_SIMP_TAC std_ss [GSYM pred_setTheory.MEMBER_NOT_EMPTY] >>
-  EXISTS_TAC ``ms'':'a`` >>
-  FULL_SIMP_TAC std_ss [pred_setTheory.SPECIFICATION]
+rpt strip_tac >>
+fs [] >>
+rpt strip_tac >>
+(* We first prove that one iteration works (first antecedent of induction hypothesis):
+ * OK since C1 holds in ms, then use loop judgment to obtain
+ * witness *)
+subgoal `loop_step m ms var l le invariant C1 <> {}` >- (
+  simp [loop_step_def, LET_DEF] >>
+  fs [abstract_loop_jgmt_def] >>
+  QSPECL_X_ASSUM ``!x. _`` [`(var ms):num`] >>
+  fs [abstract_jgmt_def] >>
+  QSPECL_X_ASSUM ``!ms. _`` [`ms`] >>
+  rfs [] >>
+  fs [GSYM pred_setTheory.MEMBER_NOT_EMPTY] >>
+  qexists_tac `ms'':'a` >>
+  fs [pred_setTheory.SPECIFICATION]
 ) >>
-FULL_SIMP_TAC std_ss [] >>
-
-Q.ABBREV_TAC `MS' = (loop_step m ms var l le invariant C1)` >>
+(* There first four antecedents of the induction hypothesis are now in place *)
+fs [] >>
+(* Let ms' be the state at the next loop iteration *)
+Q.ABBREV_TAC `MS' = loop_step m ms var l le invariant C1` >>
 Q.ABBREV_TAC `ms' = CHOICE MS'` >>
+subgoal `loop_step m ms var l le invariant C1 ms'` >- (
+  fs [Abbr `ms'`] >>
+  ONCE_REWRITE_TAC [GSYM pred_setTheory.SPECIFICATION] >>
+  metis_tac [pred_setTheory.CHOICE_DEF]
+) >>
+(* We then prove that the invariant is preserved and loop
+ * point is l
+ * (follows from ms' being the result of a loop_step) *)
+subgoal `invariant ms' /\ (m.pc ms') = l` >- (
+  fs [loop_step_def, LET_DEF]
+) >>
+fs [] >>
+(* C1 holding in ms' remains to prove for the induction hypothesis.
+ * However, if C1 does not hold in ms', the loop exit contract can be used to
+ * complete the proof directly, so a case split is done.
+ * For both cases, weak_comp_thm is used to connect ms to ms'' via ms'. *)
+Cases_on `~C1 ms'` >| [
+  fs [loop_step_def, LET_DEF, abstract_jgmt_def] >>
+  QSPECL_X_ASSUM  ``!ms. _`` [`ms'`] >>
+  rfs [],
 
-(* We prove that the invariant is preserved *)
-SUBGOAL_THEN ``(loop_step m ms var l le invariant C1) ms'`` ASSUME_TAC >- (
-  FULL_SIMP_TAC std_ss [Abbr `ms'`] >>
-  ASSUME_TAC (ISPEC ``MS':'a->bool`` pred_setTheory.CHOICE_DEF) >>
-  REV_FULL_SIMP_TAC std_ss [pred_setTheory.SPECIFICATION]
-) >>
-Q.SUBGOAL_THEN `invariant ms'` ASSUME_TAC >- (
-  FULL_SIMP_TAC std_ss [ loop_step_def, LET_DEF]
-) >>
-FULL_SIMP_TAC std_ss [] >>
-Q.SUBGOAL_THEN `(m.pc ms') = l` ASSUME_TAC >- (
-  FULL_SIMP_TAC std_ss [ loop_step_def, LET_DEF]
-) >>
-FULL_SIMP_TAC std_ss [] >>
-
-(* If we exit the loop *)
-Cases_on `~ (C1 ms')` >- (
-  (FULL_SIMP_TAC std_ss [loop_step_def, LET_DEF]) >>
-  (FULL_SIMP_TAC std_ss [abstract_jgmt_def]) >>
-  QSPECL_X_ASSUM  ``!x. _`` [`ms'`] >>
-  (REV_FULL_SIMP_TAC std_ss []) >>
-  ASSUME_TAC (Q.SPECL [`m`] weak_comp_thm) >>
-  REV_FULL_SIMP_TAC std_ss [] >>
-  QSPECL_X_ASSUM ``!x. _`` [`ms`, `{l}`, `le`, `ms'`, `ms''`] >>
-  REV_FULL_SIMP_TAC (std_ss) [SINGLETONS_UNION_thm] >>
-  Q.SUBGOAL_THEN `l NOTIN le` (FULLSIMP_BY_THM std_ss) >- (
-    FULL_SIMP_TAC std_ss [abstract_loop_jgmt_def, pred_setTheory.IN_SING]
+  fs [loop_step_def, LET_DEF]
+] >> (
+  `m.weak ms le ms''` suffices_by (
+    metis_tac []
   ) >>
-  METIS_TAC []
-) >> (
-  FULL_SIMP_TAC std_ss []
-) >> (
-  FULL_SIMP_TAC std_ss [loop_step_def, LET_DEF]
-) >>
-ASSUME_TAC (Q.SPECL [`m`] weak_comp_thm) >>
-REV_FULL_SIMP_TAC std_ss [] >>
-QSPECL_X_ASSUM ``!x. _`` [`ms`, `{l}`, `le`, `ms'`, `ms''`] >>
-REV_FULL_SIMP_TAC (std_ss) [SINGLETONS_UNION_thm] >>
-  Q.SUBGOAL_THEN `l NOTIN le` (FULLSIMP_BY_THM std_ss) >- (
-    FULL_SIMP_TAC std_ss [abstract_loop_jgmt_def, pred_setTheory.IN_SING]
-  ) >>
-  METIS_TAC []
+  irule weak_comp_thm >>
+  fs [] >>
+  qexistsl_tac [`{l}`, `ms'`] >>
+  Q.SUBGOAL_THEN `l NOTIN le` (fn thm => fs [thm]) >- (
+    fs [abstract_loop_jgmt_def, pred_setTheory.IN_SING]
+  )
+)
 );
 
-
-
-
-val abstract_loop_rule_tmp_thm = 
-MP 
-(Q.SPEC `(\m ms var l le invariant C1.
-weak_model m ==>
-abstract_loop_jgmt m l le invariant C1 var ==>
-abstract_jgmt m l le (\ms. (invariant ms) /\ (~(C1 ms))) post ==>
-((invariant ms) /\ ((m.pc ms) = l) /\ (C1 ms)) ==>
- (?ms'. ((m.weak ms le ms') /\ (post ms'))))` loop_fun_ind) inductive_invariant;
+(* Now just some final touches to get the theorem in the exact shape we want *)
+val abstract_loop_rule_tmp_thm = MP loop_fun_ind_spec inductive_invariant;
 
 val abstract_loop_rule_thm = store_thm("abstract_loop_rule_thm",
   ``!m.
     weak_model m ==>
     !l le invariant C1 var post.
     abstract_loop_jgmt m l le invariant C1 var ==>
-    abstract_jgmt m l le (\ms. (invariant ms) /\ (~(C1 ms))) post ==>
+    abstract_jgmt m l le (\ms. invariant ms /\ ~C1 ms) post ==>
     abstract_jgmt m l le invariant post``,
 
-REPEAT STRIP_TAC >>
-SIMP_TAC std_ss [abstract_jgmt_def] >>
-REPEAT STRIP_TAC >>
+rpt strip_tac >>
+simp [abstract_jgmt_def] >>
+rpt strip_tac >>
 ASSUME_TAC (Q.SPECL [`m`, `ms`, `var`, `l`, `le`, `invariant`, `C1`] abstract_loop_rule_tmp_thm) >>
-FULL_SIMP_TAC std_ss [] >>
-REV_FULL_SIMP_TAC std_ss [] >>
+rfs [] >>
 Cases_on `C1 ms` >- (
-  FULL_SIMP_TAC std_ss [] >>
-  Q.EXISTS_TAC `ms'`>>
-  FULL_SIMP_TAC std_ss []
+  metis_tac []
 ) >>
-FULL_SIMP_TAC std_ss [abstract_jgmt_def] 
+fs [abstract_jgmt_def]
 );
 
 val _ = export_theory();
